VendingMachine/Proofs_R3.thy
@@ -1,0 +1,38 @@
+theory Proofs_R3
+  imports ExtraInv_R3 Requirements
+begin
+
+definition inv3 where "inv3 s \<equiv> extraInv s \<and> R3 s"
+
+lemmas einv_rule = P6_5_rule
+lemmas req_rule = P6_5_einv2req
+
+theorem extra1: "VC1 extraInv s0"
+  apply(unfold VC1_def extraInv_def commonExtraInv_def P6_5inv_def P6_2inv_def always2_inv_def weak_until_inv_def
+always_def previous_ex_def)
+  apply auto
+  done
+
+theorem extra9: "VC9 extraInv env s0 button1'value button2'value deposited'value given1'value given2'value paidOut'value
+ cancel'value "
+apply(unfold VC9_def extraInv_def)
+ apply(rule impI)
+  apply(rule conjI)
+  using cei9 apply((auto simp add: VC9_def)[1];fastforce)
+  apply(unfold commonExtraInv_def)
+  apply(erule conjE)+
+  apply(erule einv_rule)
+   apply(auto split: if_splits)
+  done
+
+theorem extra72: "VC72 extraInv env s0 button1'value button2'value deposited'value given1'value given2'value paidOut'value
+ cancel'value "
+apply(unfold VC72_def extraInv_def)
+ apply(rule impI)
+  apply(rule conjI)
+  using cei72 apply((auto simp add: VC72_def)[1];fastforce)
+  apply(unfold commonExtraInv_def)
+  apply(erule conjE)+
+  apply(erule einv_rule)
+   apply(auto split: if_splits)
+  done
